Common/Exec.v
@@ -360,7 +360,7 @@ Proof.
   elim l; cdestruct |- ***; set_solver.
 Qed.
 
-#[global] Instance res_unfold:elem_of_mthrow {St E A} x (err : E) st :
+#[global] Instance res_unfold_elem_of_mthrow {St E A} x (err : E) st :
   UnfoldElemOf x ((mthrow err : Exec.t St E A) st) False.
 Proof. tcclean. unfold mthrow, throw_inst, mthrow, res_throw_inst. set_solver. Qed.
 
